examples/modfair/ModFairNot.v
@@ -1,0 +1,71 @@
+Require Import Coqlib.
+Require Import ITreelib.
+Require Import ImpPrelude.
+Require Import STS.
+Require Import Behavior.
+Require Import ModSem.
+Require Import Skeleton.
+Require Import PCM.
+Require Import HoareDef STB IPM.
+Require Import sProp sWorld World SRF.
+Require Import ProofMode IProofMode.
+
+Require Import FairCounter WFLibLarge.
+
+Set Implicit Arguments.
+
+
+Section A.
+
+  Context `{_W: CtxWD.t}.
+
+  Variable id: ID.
+  Variable wf: WF.
+
+  Variable initial_map: iimap id wf.
+
+  Definition unfairF: list (id -> Flag.t) -> itree hEs val :=
+    fun _ =>
+      Ret Vundef.
+
+  Definition unfair_spec: fspec :=
+    mk_fspec_inv 0
+      (fun _ _ => 
+        mk_simple (X := nat)
+          (fun (k: nat) =>
+            (ord_top,
+            (fun varg => (⌜exists ff: id -> Flag.t, varg = [ff]↑⌝)%I),
+            (fun _ => (True)%I)))).
+
+  Definition UnFairStb: list (gname * fspec).
+    eapply (Seal.sealing "stb").
+    apply [("fair", unfair_spec)].
+  Defined.
+
+  Definition UnFairSbtb: list (string * fspecbody) :=
+    [("fair", mk_specbody unfair_spec (cfunU unfairF))].
+
+  Definition SUnFairSem: SModSem.t := {|
+    SModSem.fnsems := UnFairSbtb;
+    SModSem.initial_cond := emp;
+    SModSem.initial_st := initial_map↑;
+  |}
+  .
+
+  Definition SUnFair: SMod.t := {|
+    SMod.get_modsem := fun _ => SUnFairSem;
+    SMod.sk := [("fair", Gfun↑)];
+  |}
+  .
+
+  Variable GlobalStb: Sk.t -> gname -> option fspec.
+  Definition _HUnFair: HMod.t := (SMod.to_hmod GlobalStb SUnFair).
+  Definition HUnFair := _HUnFair.
+
+  Lemma HUnFair_unfold: HUnFair = _HUnFair.
+  Proof. eauto. Qed.
+
+  Global Opaque HUnFair.
+
+End A.
+Global Hint Unfold UnFairStb: stb.
